error on method_instance

Simu/Syn.v
@@ -52,14 +52,6 @@ Inductive stmt : Type :=
     list (ident * typ) -> ident -> ident -> ident -> list exp -> stmt 
 | Skip.                  (*  *)
 
-Fixpoint instance_methods (s: stmt): list (ident * ident * ident) :=
-  match s with
-  | Ifte _ s1 s2  
-  | Comp s1 s2 => instance_methods s2 ++ instance_methods s1
-  | Call _ cls o f _ => [(o, cls, f)] 
-  | _ => []
-  end.
-
 Inductive VarsDeclared_exp (vars: list (ident * typ)): exp -> Prop :=
 | vd_var: forall x ty,
     In (x, ty) vars ->
